\begin{tcolorbox}[sharp corners, colback=white,boxrule=1mm]
	$P \wedge P = P$

	$P \vee P = P$
	
	$P \wedge Q = Q \wedge P$
	
	$P \vee Q = Q \vee P$
	
	$P \leftrightarrow Q = Q \leftrightarrow P$
	
	$P \leftrightarrow Q = (P \rightarrow Q) \wedge (Q \rightarrow P)$
	
	$P \rightarrow Q = \neg Q \rightarrow \neg P$
	
	$P \rightarrow Q = \neg P \vee Q$
	
	$P \wedge (P \vee Q) = P \vee (P \wedge Q)$
	
	Todo A não é B = Nenhum A é B
	
	Nenhum A não é B = Todo A é B
	
	Leis associativas:
	\begin{itemize}
		\item $(P \wedge Q) \wedge S = P \wedge (Q \wedge S)$
		\item $(P \vee Q) \vee S = P \vee (Q \vee S)$
	\end{itemize}

	Leis distributivas:
	\begin{itemize}
		\item $P \wedge (Q \vee S) = (P \wedge Q) \vee (P \wedge S)$
		\item $P \vee (Q \wedge S) = (P \vee Q) \wedge (P \vee S)$
	\end{itemize}

	Lei da dupla negação:
	$\neg(\neg P) = P$
	
	$\neg (P \wedge Q) = \neg P \vee \neg Q$
	
	$\neg (P \vee Q) = \neg P \wedge \neg Q$
	
	$\neg (P \rightarrow Q) = P \wedge \neg Q$
	
	\begin{tabular}{|c|c|}
		\hline 
		Proposição & Negação da proposição \\ 
		\hline 
		Algum... & Nenhum... \\ 
		\hline 
		Nenhum... & Algum... \\ 
		\hline 
		Todo... & Algum ... não... \\ 
		\hline 
	\end{tabular} 
\end{tcolorbox}